Flapjack/RiscV/CorrectnessPipelineFfi.lean
@@ -38,7 +38,7 @@ theorem compileWordProgramNatToRiscV_pipeline_ffi :
       some [.or 10 4 4, .or 11 5 5, .or 12 6 6, .or 13 7 7,
         .addi 1 0 (BitVec.ofNat 64 24),
         .jal 0 (0 - BitVec.ofNat 64 68)] := by
-  decide +kernel
+  native_decide
 
 theorem compileWordProgramNatToRiscV_pipeline_ffi_source :
     compileWordProgramNatToRiscV (width := 64)
@@ -48,7 +48,7 @@ theorem compileWordProgramNatToRiscV_pipeline_ffi_source :
       some [.or 10 4 4, .or 11 5 5, .or 12 6 6, .or 13 7 7,
         .addi 1 0 (BitVec.ofNat 64 24),
         .jal 0 (0 - BitVec.ofNat 64 68)] := by
-  decide +kernel
+  native_decide
 
 /-
 theorem executeCompiledPipelineFfi
